
$$\forall \phi(x) \Rightarrow \exists_{x} \phi (x)$$
$$\neg \forall_{x}\phi (x)\Rightarrow \exists_x\neg\phi(x)$$
$$\neg \exists_x\phi(x)\Leftrightarrow\forall_{x}\neg \phi(x)$$
$$\forall_x(\phi(x)\land\psi(x))\Leftrightarrow \exists_{x}\phi (x) \lor\exists_x\psi(x)$$
$$\exists_x(\phi(x)\lor\psi(x))\Leftrightarrow\exists_x\phi(x)\land\exists_x\psi(x)$$
$$\exists_x(\phi(x)\psi(x))\Rightarrow\exists_x\phi(x)\lor\exists_x\psi(x)$$
$$\forall_x(\phi(x)\lor\forall_x\psi(x))\Rightarrow\forall_x(\phi(x)\lor\psi(x))$$
$$\forall_x\forall_y\phi(x,y)\Leftrightarrow\exists_x\exists_y\phi(x,y)$$
$$\exists_x\exists_y\phi(x,y)\Leftrightarrow\exists_x\exists_y\phi(x,y)$$
$$\exists_x\forall_y\phi(x,y)\Rightarrow\forall_y\exists_x\phi(x,y)$$